ECCA_typing.v
@@ -13,63 +13,68 @@ Inductive ECCA_sub_type: ECCAenv -> ECCAexp -> ECCAexp -> Prop :=
   ECCA_sub_type g A B
 | aST_Cum (g: ECCAenv) (i: nat) :
   ECCA_sub_type g (eUni (uType i)) (eUni (uType (S i)))
-| aST_Pi (g: ECCAenv) (A1 A2 B1 B2: ECCAexp) (x1 x2: atom) :
+| aST_Pi (g: ECCAenv) (A1 A2 B1 B2: ECCAexp) (x: name) :
   (ECCA_Equiv g A1 A2) ->
-  (ECCA_sub_type (Assum g x1 A2) B1 (subst x2 (eId x1) B2)) -> (* eId x1 ?*)
-  (ECCA_sub_type g (ePi x1 A1 B1) (ePi x2 A2 B2))
+  (ECCA_sub_type (g & x ~ Assum A2) (open x B1) (open x B2)) -> (* eId x1 ?*)
+  (ECCA_sub_type g (ePi A1 B1) (ePi A2 B2))
 | aST_Trans (g: ECCAenv) (A A' B: ECCAexp) :
   (ECCA_sub_type g A A') ->
   (ECCA_sub_type g A' B) ->
   (ECCA_sub_type g A B)
 | aST_Prop (g: ECCAenv) :
   (ECCA_sub_type g (eUni (uProp)) (eUni (uType 0)))
-| aST_Sig (g: ECCAenv) (A1 A2 B1 B2: ECCAexp) (x1 x2: atom):
+| aST_Sig (g: ECCAenv) (A1 A2 B1 B2: ECCAexp) (x: name):
   (ECCA_sub_type g A1 A2) ->
-  (ECCA_sub_type (Assum g x1 A2) B1 (subst x2 (eId x1) B2)) ->
-  (ECCA_sub_type g (eSig x1 A1 B1) (eSig x2 A2 B2))
+  (ECCA_sub_type (g & x ~ Assum A2) (open x B1) (open x B2)) ->
+  (ECCA_sub_type g (eSig A1 B1) (eSig A2 B2))
 .
 Hint Constructors ECCA_sub_type.
 
 Reserved Notation "g '|-' a ':' b" (at level 250, a at level 99).
 Inductive ECCA_has_type: ECCAenv -> ECCAexp -> ECCAexp -> Prop :=
 | aT_Ax_Prop (g: ECCAenv) :
+  ECCA_Env_WF g ->
   (g |- (eUni uProp) : (eUni (uType 0)))
 | aT_Ax_Type (g: ECCAenv) (i: nat) :
+  ECCA_Env_WF g ->
   (g |- (eUni (uType i)) : (eUni (uType (S i))))
 | aT_Var (g: ECCAenv) (x: atom) (A: ECCAexp) :
-  (ECCA_LookupTypeR g x A) -> (* this needs adjustment *)
+  (assumes g x A) -> (* this needs adjustment *)
   (g |- (eId x) : A)
 | aT_Bool (g: ECCAenv):
+  ECCA_Env_WF g ->
   (g |- (eBool) : (eUni (uType 0)))
 | aT_True (g: ECCAenv):
+  ECCA_Env_WF g ->
   (g |- (eTru) : (eBool))
 | aT_False (g: ECCAenv):
+  ECCA_Env_WF g ->
   (g |- (eFls) : (eBool)) 
-| aT_Sig (g: ECCAenv) (x: atom) (A B: ECCAexp) (i: nat) :
+| aT_Sig (g: ECCAenv) (x: name) (A B: ECCAexp) (i: nat) :
   (g |- A : (eUni (uType i))) ->
-  (ECCA_has_type (Assum g x A) B (eUni (uType i))) ->
-  (g |- (eSig x A B) : (eUni (uType i)))
-| aT_Pair (g: ECCAenv) (v1 v2: ECCAexp) (A B: ECCAexp) (x: atom) :
+  (ECCA_has_type (g & x ~ Assum A) (open x B) (eUni (uType i))) ->
+  (g |- (eSig A B) : (eUni (uType i)))
+| aT_Pair (g: ECCAenv) (v1 v2: ECCAexp) (A B: ECCAexp) :
   (g |- v1 : A) ->
-  (g |- v2 : (subst x v1 B)) ->
-  (g |- (ePair v1 v2 (eSig x A B)) : (eSig x A B))
-| aT_Prod_Prop (g: ECCAenv) (x: atom) (A B: ECCAexp) (i: nat):
+  (g |- v2 : (bind v1 B)) ->
+  (g |- (ePair v1 v2 (eSig A B)) : (eSig A B))
+| aT_Prod_Prop (g: ECCAenv) (x: name) (A B: ECCAexp) (i: nat):
   (g |- A : (eUni (uType i))) ->
-  (ECCA_has_type (Assum g x A) B (eUni (uProp))) ->
-  (g |- (ePi x A B) : (eUni (uProp)))
-| aT_Prod_Type (g: ECCAenv) (x: atom) (A B: ECCAexp) (i: nat):
+  (ECCA_has_type (g & x ~ Assum A) (open x B) (eUni (uProp))) ->
+  (g |- (ePi A B) : (eUni (uProp)))
+| aT_Prod_Type (g: ECCAenv) (x: name) (A B: ECCAexp) (i: nat):
   (g |- A : (eUni (uType i))) ->
-  (ECCA_has_type (Assum g x A) B (eUni (uType i))) ->
-  (g |- (ePi x A B) : (eUni (uType i)))
-| aT_Lam (g: ECCAenv) (x: atom) (A e B: ECCAexp) :
-  (ECCA_has_type (Assum g x A) e B) ->
-  (g |- (eAbs x A e) : (ePi x A B))
+  (ECCA_has_type (g & x ~ Assum A) (open x B) (eUni (uType i))) ->
+  (g |- (ePi A B) : (eUni (uType i)))
+| aT_Lam (g: ECCAenv) (x: name) (A e B: ECCAexp) :
+  (ECCA_has_type (g & x ~ Assum A) (open x e) (open x B)) ->
+  (g |- (eAbs A e) : (ePi A B))
 (* ECCA_has_type: ECCAenv -> ECCAconf -> ECCAconf -> Prop := *)
-| aT_Let (g: ECCAenv) (n m A B: ECCAexp) (x: atom):
+| aT_Let (g: ECCAenv) (n m A B: ECCAexp) (x: name):
   (g |- n : A) ->
 (*should this be (def(assum(g))) or (assum(def(g)))*)
-  (ECCA_has_type (Assum (Def g x n) x A) m B) ->
-  (g |- (eLet x n m) : (subst x n B))
+  (ECCA_has_type (g & x ~ Def n A) (open x m) (open x B)) ->
+  (g |- (eLet n m) : (bind n B))
 (* | aT_If (g: ECCAenv) (B U e1 e2: ECCAexp) (e: ECCAexp) (x: atom):
   ECCA_has_type (Assum g x eBool) B U -> 
   g |- e : eBool ->
@@ -82,16 +87,16 @@ Inductive ECCA_has_type: ECCAenv -> ECCAexp -> ECCAexp -> Prop :=
   (ECCA_sub_type g A B) ->
   (g |- e : B)
 (* ECCA_has_type: ECCAenv -> ECCAcomp -> ECCAconf -> Prop := *)
-| aT_App (g: ECCAenv) (x: atom) (e e': ECCAexp) (A' B: ECCAexp) :
-  (g |- e : (ePi x A' B)) ->
+| aT_App (g: ECCAenv) (x: name) (e e': ECCAexp) (A' B: ECCAexp) :
+  (g |- e : (ePi A' B)) ->
   (g |- e' : A') ->
-  (g |- (eApp e e') : (subst x e B))
-| aT_Fst (g: ECCAenv) (e: ECCAexp) (A B: ECCAexp) (x: atom) :
-  (g |- e: (eSig x A B)) ->
+  (g |- (eApp e e') : (bind e B))
+| aT_Fst (g: ECCAenv) (e: ECCAexp) (A B: ECCAexp) :
+  (g |- e: (eSig A B)) ->
   (g |- (eFst e): A)
-| aT_Snd (g: ECCAenv) (e: ECCAexp) (A B: ECCAexp) (x: atom) :
-  (g |- e: (eSig x A B)) ->
-  (g |- (eSnd e): (subst x (eFst e) B)) 
+| aT_Snd (g: ECCAenv) (e: ECCAexp) (A B: ECCAexp) :
+  (g |- e: (eSig A B)) ->
+  (g |- (eSnd e): (bind (eFst e) B)) 
 (* | aT_Subst (x: atom) (g: ECCAenv) (A B U: ECCAexp) (e e1 e2: ECCAexp):
   (ECCA_has_type (Assum g x A) B U) ->
   g |- e1: A -> 
@@ -100,21 +105,21 @@ Inductive ECCA_has_type: ECCAenv -> ECCAexp -> ECCAexp -> Prop :=
   ECCA_LookupEqR g e1 e2 ->
   g |- (eSubst e1 e2 e): (subst x e2 B)  *)
 where "g '|-' a ':' b" := (ECCA_has_type g a b) : ECCA_scope
-.
-Hint Constructors ECCA_has_type.
-
-(* ECC Well-Formed Environments *)
-Inductive ECCA_Env_WF: ECCAenv -> Prop :=
+with 
+(* ECCA Well-Formed Environments *)
+ECCA_Env_WF: ECCAenv -> Prop :=
 | W_Empty (g: ECCAenv) :
-  ECCA_Env_WF Empty
-| W_Assum (g: ECCAenv) (x: atom) (A U: ECCAexp) :
+  ECCA_Env_WF ctx_empty
+| W_Assum (g: ECCAenv) (x: name) (A U: ECCAexp) :
   ECCA_Env_WF g ->
   ECCA_has_type g A U ->
-  ECCA_Env_WF (Assum g x A)
-| W_Def (g: ECCAenv) (x: atom) (e A U: ECCAexp) :
+  ECCA_Env_WF (g & x ~ Assum A)
+| W_Def (g: ECCAenv) (x: name) (e A U: ECCAexp) :
   ECCA_Env_WF g ->
   ECCA_has_type g A U ->
   ECCA_has_type g e A ->
-  ECCA_Env_WF (Assum (Def g x e) x A)
+  ECCA_Env_WF (g & x ~ Def e A)
+(* | W_Eq  *)
 .
+Hint Constructors ECCA_has_type.
 Hint Constructors ECCA_Env_WF.
